refine: arch-split ADT_H (AARCH64 ONLY)
In order to increase type signature compatibility between architectures,
we recognise the FPU owner parameter even on architectures which don't
have FPU (by setting the parameter to False).

The bulk of the remaining arch-specific proof is absHeap_correct, whose
current design leans heavily on digging into arch-related concepts. To
get a better arch-split, this proof would have to be thoroughly
re-designed.

Signed-off-by: Rafal Kolanski <rafal.kolanski@proofcraft.systems>

proof/refine/ADT_H.thy
@@ -11,13 +11,14 @@ theory ADT_H
   imports ArchSyscall_R (* FIXME arch-split: "AInvs.ADT_AI" *)
 begin
 
+arch_requalify_facts pageBitsForSize_bounded (* FIXME arch-split: ArchInvariants_AI *)
+
 text \<open>
   The general refinement calculus (see theory Simulation) requires
   the definition of a so-called ``abstract datatype'' for each refinement layer.
   This theory defines this datatype for the executable specification.
   It is based on the abstract specification because we chose
-  to base the refinement's observable state on the abstract state.
-\<close>
+  to base the refinement's observable state on the abstract state.\<close>
 
 consts
   initEntry :: machine_word
@@ -27,13 +28,10 @@ consts
   initBootFrames :: "machine_word list"
   initDataStart :: machine_word
 
-context begin interpretation Arch . (*FIXME: arch-split*)
-
 text \<open>
   The construction of the abstract data type
   for the executable specification largely follows
-  the one for the abstract specification.
-\<close>
+  the one for the abstract specification.\<close>
 definition Init_H :: "kernel_state global_state set" where
   "Init_H \<equiv>
     ({empty_context} \<times> snd `
@@ -50,71 +48,6 @@ definition
   "device_mem' s \<equiv> \<lambda>p.
      if pointerInDeviceData p s then Some p else None"
 
-definition vm_rights_of :: "vmrights \<Rightarrow> rights set" where
-  "vm_rights_of x \<equiv> case x of VMKernelOnly \<Rightarrow> vm_kernel_only
-                    | VMReadOnly \<Rightarrow> vm_read_only
-                    | VMReadWrite \<Rightarrow> vm_read_write"
-
-lemma vm_rights_of_vmrights_map_id[simp]:
-  "rs \<in> valid_vm_rights \<Longrightarrow> vm_rights_of (vmrights_map rs) = rs"
-  by (auto simp: vm_rights_of_def vmrights_map_def valid_vm_rights_def
-                 vm_read_write_def vm_read_only_def vm_kernel_only_def)
-
-(* We expect 'a to be one of {pt_index, vs_index} *)
-definition absPageTable0 ::
-  "(obj_ref \<rightharpoonup> Structures_H.kernel_object) \<Rightarrow> obj_ref \<Rightarrow> 'a::len word \<rightharpoonup> AARCH64_A.pte" where
-  "absPageTable0 h a \<equiv> \<lambda>offs.
-   case h (a + (ucast offs << pte_bits)) of
-     Some (KOArch (KOPTE (InvalidPTE))) \<Rightarrow> Some AARCH64_A.InvalidPTE
-   | Some (KOArch (KOPTE (PagePTE p small global execNever dev rights))) \<Rightarrow>
-       Some (AARCH64_A.PagePTE p small
-                               {x. global \<and> x=Global \<or> \<not>execNever \<and> x = Execute \<or>
-                                   dev \<and> x = Device}
-                               (vm_rights_of rights))
-   | Some (KOArch (KOPTE (PageTablePTE p))) \<Rightarrow>
-       if p \<le> mask ppn_len
-       then Some (AARCH64_A.PageTablePTE (ucast p))
-       else None
-   | _ \<Rightarrow> None"
-
-definition absPageTable ::
-  "(obj_ref \<rightharpoonup> Structures_H.kernel_object) \<Rightarrow> pt_type option \<Rightarrow> obj_ref \<rightharpoonup> pt" where
-  "absPageTable h pt_t a \<equiv>
-   case pt_t of
-     Some NormalPT_T \<Rightarrow>
-       if is_aligned a (pt_bits NormalPT_T) \<and> (\<forall>off::pt_index. absPageTable0 h a off \<noteq> None)
-       then Some (NormalPT (\<lambda>off. the (absPageTable0 h a off)))
-       else None
-   | Some VSRootPT_T \<Rightarrow>
-       if is_aligned a (pt_bits VSRootPT_T) \<and> (\<forall>off::vs_index. absPageTable0 h a off \<noteq> None)
-       then Some (VSRootPT (\<lambda>off. the (absPageTable0 h a off)))
-       else None
-   | None \<Rightarrow> None"
-
-definition absVGIC :: "gicvcpuinterface \<Rightarrow> gic_vcpu_interface" where
-  "absVGIC v \<equiv> case v of
-    VGICInterface hcr vmcr apr lr \<Rightarrow> gic_vcpu_interface.make hcr vmcr apr lr"
-
-lemma absVGIC_eq[simp]:
-  "absVGIC (vgic_map vgic) = vgic"
-  by (simp add: vgic_map_def absVGIC_def gic_vcpu_interface.make_def)
-
-(* Can't pull the whole heap off at once, start with arch specific stuff.*)
-definition absHeapArch ::
-  "(machine_word \<rightharpoonup> kernel_object) \<Rightarrow> (machine_word \<rightharpoonup> pt_type) \<Rightarrow>
-   machine_word \<Rightarrow> arch_kernel_object \<rightharpoonup> arch_kernel_obj" where
-  "absHeapArch h pt_types a \<equiv> \<lambda>ako.
-     case ako of
-       KOASIDPool (AARCH64_H.ASIDPool ap) \<Rightarrow>
-         Some (AARCH64_A.ASIDPool (\<lambda>w. map_option abs_asid_entry (ap (ucast w))))
-     | KOPTE _ \<Rightarrow>
-         map_option PageTable (absPageTable h (pt_types a) a)
-     | KOVCPU (VCPUObj tcb vgic regs vppimask) \<Rightarrow>
-       Some (VCPU \<lparr> vcpu_vgic   = absVGIC vgic,
-                    vcpu_regs   = regs,
-                    vcpu_tcb    = tcb,
-                    vcpu_vppi_masked = vppimask \<rparr>)"
-
 definition
   "EndpointMap ep \<equiv> case ep of
                      Structures_H.IdleEP \<Rightarrow> Structures_A.IdleEP
@@ -129,13 +62,25 @@ definition
                      | Structures_H.ActiveNtfn b \<Rightarrow> Structures_A.ActiveNtfn b
       , ntfn_bound_tcb = ntfnBoundTCB ntfn \<rparr>"
 
-definition mdata_map' ::
-  "(asid \<times> vspace_ref) option \<Rightarrow> (Machine_A.AARCH64_A.asid \<times> vspace_ref) option" where
-  "mdata_map' = map_option (\<lambda>(asid, ref). (ucast asid, ref))"
-
-lemma mdata_map'_inv[simp]:
-  "mdata_map' (mdata_map m) = m"
-  by (cases m; simp add: mdata_map_def mdata_map'_def split_def ucast_down_ucast_id is_down)
+locale ADT_H =
+  fixes vm_rights_of :: "vmrights \<Rightarrow> rights set"
+  fixes ArchCapabilityMap :: "arch_capability \<Rightarrow> cap"
+  fixes ArchFaultMap :: "Fault_H.arch_fault \<Rightarrow> ExceptionTypes_A.arch_fault"
+  (* the boolean argument is whether the TCB is the current FPU owner; on non-FPU architectures
+     this is ignored, but the common type allows a generic phrasing of TcbMap *)
+  fixes ArchTcbMap :: "Structures_H.arch_tcb \<Rightarrow> bool \<Rightarrow> Structures_A.arch_tcb"
+  fixes absArchState ::
+    "Arch.kernel_state \<Rightarrow> (obj_ref \<Rightarrow> arch_kernel_object option) \<Rightarrow> arch_state"
+  assumes vm_rights_of_vmrights_map_id[simp]:
+    "\<And>rs. rs \<in> valid_vm_rights \<Longrightarrow> vm_rights_of (vmrights_map rs) = rs"
+  assumes acap_relation_imp_ArchCapabilityMap:
+    "\<And>ac ac'.
+     \<lbrakk>wellformed_acap ac; acap_relation ac ac'\<rbrakk> \<Longrightarrow> ArchCapabilityMap ac' = cap.ArchObjectCap ac"
+  assumes ArchFaultMap_arch_fault_map:
+    "\<And>f. ArchFaultMap (arch_fault_map f) = f"
+  assumes absArchState_correct:
+    "\<And>s s'. (s,s') \<in> state_relation \<Longrightarrow> absArchState (ksArchState s') (aobjs_of' s') = arch_state s"
+begin
 
 fun CapabilityMap :: "capability \<Rightarrow> cap" where
   "CapabilityMap capability.NullCap = cap.NullCap"
@@ -155,25 +100,7 @@ fun CapabilityMap :: "capability \<Rightarrow> cap" where
 | "CapabilityMap (capability.IRQHandlerCap irq) = cap.IRQHandlerCap irq"
 | "CapabilityMap (capability.Zombie p b n) =
    cap.Zombie p (case b of ZombieTCB \<Rightarrow> None | ZombieCNode n \<Rightarrow> Some n) n"
-| "CapabilityMap (capability.ArchObjectCap (arch_capability.ASIDPoolCap x y)) =
-   cap.ArchObjectCap (arch_cap.ASIDPoolCap x (ucast y))"
-| "CapabilityMap (capability.ArchObjectCap (arch_capability.ASIDControlCap)) =
-   cap.ArchObjectCap (arch_cap.ASIDControlCap)"
-| "CapabilityMap (capability.ArchObjectCap
-                    (arch_capability.FrameCap word rghts sz d data)) =
-   cap.ArchObjectCap (arch_cap.FrameCap word (vm_rights_of rghts) sz d (mdata_map' data))"
-| "CapabilityMap (capability.ArchObjectCap
-                    (arch_capability.PageTableCap word pt_t data)) =
-  cap.ArchObjectCap (arch_cap.PageTableCap word pt_t (mdata_map' data))"
-| "CapabilityMap (capability.ArchObjectCap
-                    (arch_capability.VCPUCap v)) =
-  cap.ArchObjectCap (arch_cap.VCPUCap v)"
-| "CapabilityMap (capability.ArchObjectCap
-                    (arch_capability.SGISignalCap irq target)) =
-  cap.ArchObjectCap (arch_cap.SGISignalCap (ucast irq) (ucast target))"
-| "CapabilityMap (capability.ArchObjectCap
-                    (arch_capability.SMCCap smc_badge)) =
-  cap.ArchObjectCap (arch_cap.SMCCap smc_badge)"
+| "CapabilityMap (capability.ArchObjectCap acap) = ArchCapabilityMap acap"
 
 (* FIXME: wellformed_cap_simps has lots of duplicates. *)
 lemma cap_relation_imp_CapabilityMap:
@@ -189,9 +116,10 @@ lemma cap_relation_imp_CapabilityMap:
     apply (simp add: uint_of_bl_is_bl_to_bin bl_bin_bl[simplified])
    apply (simp add: zbits_map_def split: option.splits)
   apply (rename_tac arch_cap)
-  apply clarsimp
-  apply (case_tac arch_cap; simp add: wellformed_cap_simps ucast_down_ucast_id is_down)
+  apply (clarsimp simp: acap_relation_imp_ArchCapabilityMap)
   done
+
+end (* ADT_H *)
 
 primrec ThStateMap :: "Structures_H.thread_state \<Rightarrow> Structures_A.thread_state" where
   "ThStateMap Structures_H.thread_state.Running =
@@ -238,11 +166,7 @@ lemma LookupFailureMap_lookup_failure_map:
                simp del: bin_to_bl_def
                split: ExceptionTypes_A.lookup_failure.splits)
 
-primrec ArchFaultMap :: "Fault_H.arch_fault \<Rightarrow> ExceptionTypes_A.arch_fault" where
-  "ArchFaultMap (AARCH64_H.VMFault p m) = AARCH64_A.VMFault p m"
-| "ArchFaultMap (AARCH64_H.VCPUFault w) = AARCH64_A.VCPUFault w"
-| "ArchFaultMap (AARCH64_H.VGICMaintenance m) = AARCH64_A.VGICMaintenance m"
-| "ArchFaultMap (AARCH64_H.VPPIEvent irq) = AARCH64_A.VPPIEvent irq"
+context ADT_H begin
 
 primrec FaultMap :: "Fault_H.fault \<Rightarrow> ExceptionTypes_A.fault" where
   "FaultMap (Fault_H.fault.CapFault ref b failure) =
@@ -254,24 +178,12 @@ primrec FaultMap :: "Fault_H.fault \<Rightarrow> ExceptionTypes_A.fault" where
 | "FaultMap (Fault_H.fault.UserException x y) =
      ExceptionTypes_A.fault.UserException x y"
 
-lemma ArchFaultMap_arch_fault_map: "ArchFaultMap (arch_fault_map f) = f"
-  by (cases f; simp add: ArchFaultMap_def arch_fault_map_def)
-
 lemma FaultMap_fault_map[simp]:
   "valid_fault ft \<Longrightarrow> FaultMap (fault_map ft) = ft"
   apply (case_tac ft, simp_all)
    apply (simp add: valid_fault_def LookupFailureMap_lookup_failure_map)
   apply (rule ArchFaultMap_arch_fault_map)
   done
-
-definition
-  "ArchTcbMap atcb is_cur_fpu_owner \<equiv>
-    \<lparr> tcb_context = atcbContext atcb, tcb_vcpu = atcbVCPUPtr atcb, tcb_cur_fpu = is_cur_fpu_owner \<rparr>"
-
-lemma arch_tcb_relation_imp_ArchTcnMap:
-  "\<lbrakk> arch_tcb_relation atcb atcb'; tcb_cur_fpu atcb = is_cur_fpu_owner\<rbrakk>
-   \<Longrightarrow> ArchTcbMap atcb' is_cur_fpu_owner = atcb"
-  by (clarsimp simp: arch_tcb_relation_def ArchTcbMap_def)
 
 definition
   "TcbMap tcb is_cur_fpu_owner \<equiv>
@@ -299,39 +211,7 @@ definition
                                 Some (KOCTE cte) \<Rightarrow> cteCap cte))
     else None)"
 
-definition absHeap ::
-  "(machine_word \<rightharpoonup> vmpage_size) \<Rightarrow> (machine_word \<rightharpoonup> nat) \<Rightarrow> (machine_word \<rightharpoonup> pt_type) \<Rightarrow>
-     (machine_word \<rightharpoonup> Structures_H.kernel_object) \<Rightarrow> machine_word option \<Rightarrow> Structures_A.kheap" where
-  "absHeap ups cns pt_types h cur_fpu_owner \<equiv> \<lambda>x.
-     case h x of
-       Some (KOEndpoint ep) \<Rightarrow> Some (Endpoint (EndpointMap ep))
-     | Some (KONotification ntfn) \<Rightarrow> Some (Notification (AEndpointMap ntfn))
-     | Some KOKernelData \<Rightarrow> undefined \<comment> \<open>forbidden by pspace_relation\<close>
-     | Some KOUserData \<Rightarrow> map_option (ArchObj \<circ> DataPage False) (ups x)
-     | Some KOUserDataDevice \<Rightarrow> map_option (ArchObj \<circ> DataPage True) (ups x)
-     | Some (KOTCB tcb) \<Rightarrow> Some (TCB (TcbMap tcb (cur_fpu_owner = Some x)))
-     | Some (KOCTE cte) \<Rightarrow> map_option (\<lambda>sz. absCNode sz h x) (cns x)
-     | Some (KOArch ako) \<Rightarrow> map_option ArchObj (absHeapArch h pt_types x ako)
-     | None \<Rightarrow> None"
-
-lemma unaligned_page_offsets_helper:
-  "\<lbrakk>is_aligned y (pageBitsForSize vmpage_size); n\<noteq>0;
-    n < 2 ^ (pageBitsForSize vmpage_size - pageBits)\<rbrakk>
-   \<Longrightarrow> \<not> is_aligned (y + n * 2 ^ pageBits :: machine_word) (pageBitsForSize vmpage_size)"
-  apply (simp (no_asm_simp) add: is_aligned_mask)
-  apply (simp add: mask_add_aligned)
-  apply (cut_tac mask_eq_iff_w2p [of "pageBitsForSize vmpage_size" "n * 2 ^ pageBits"])
-   prefer 2
-   apply (case_tac vmpage_size, simp_all add: word_size bit_simps)
-  apply (cut_tac word_power_nonzero_64[of n pageBits];
-         simp add: word_bits_conv pageBits_def)
-   prefer 2
-   apply (case_tac vmpage_size, simp_all add: bit_simps word_size)
-     apply (frule less_trans[of n _ "0x10000000000000"], simp+)+
-  apply clarsimp
-  apply (case_tac vmpage_size, simp_all add: bit_simps)
-    apply (frule_tac i=n and k="0x1000" in word_mult_less_mono1, simp+)+
-  done
+end (* ADT_H *)
 
 lemma pspace_aligned_distinct_None:
   (* NOTE: life would be easier if pspace_aligned and pspace_distinct were defined on PSpace instead of the whole kernel state. *)
@@ -356,48 +236,11 @@ lemma pspace_aligned_distinct_None:
   apply (simp add: or.assoc le_word_or2)
   apply (simp add: word_plus_and_or_coroll[symmetric])
   apply (subgoal_tac "x + y \<le> x + mask (obj_bits ko)", simp)
-  apply (rule word_add_le_mono2)
+  (* prevent leaking LENGTH *)
+  apply (rule word_add_le_mono2[where 'a=machine_word_len, folded word_bits_def])
    apply (simp add: mask_def plus_one_helper)
-  apply (thin_tac "~ P" for P)+
-  apply (thin_tac "(x::'a::len word) < y" for x y)+
-  apply (thin_tac "x = Some y" for x y)+
-  apply (thin_tac "x && mask (obj_bits ko') = 0" for x)
-  apply (thin_tac "x && y = 0")
-  apply (clarsimp simp add: dvd_def word_bits_len_of word_bits_conv
-                            and_mask_dvd_nat[symmetric])
-  apply (cut_tac x=x in unat_lt2p)
-  apply (cut_tac x="mask (obj_bits ko)::machine_word" in unat_lt2p)
-  apply (simp add: mult.commute
-                   add.commute[of "unat (mask (obj_bits ko))"])
-  apply (case_tac "k=0", simp+)
-  apply (subgoal_tac "obj_bits ko\<le>64")
-   prefer 2
-   apply (rule ccontr)
-   apply (simp add: not_le)
-   apply (frule_tac a="2::nat" and n=64 in power_strict_increasing, simp+)
-   apply (case_tac "k=1", simp)
-   apply (cut_tac m=k and n="2 ^ obj_bits ko" in n_less_n_mult_m,
-          (simp(no_asm_simp))+)
-   apply (simp only: mult.commute)
-  apply (thin_tac "x = y" for x y)+
-  apply (clarsimp simp add: le_less)
-  apply (erule disjE)
-   prefer 2
-   apply (simp add: mask_def)
-  apply (subgoal_tac "obj_bits ko <= (63::nat)", simp_all)
-  apply (simp add: mask_def unat_minus_one word_bits_conv)
-  apply (cut_tac w=k and c="2 ^ obj_bits ko" and b="2^(64-obj_bits ko)"
-              in less_le_mult_nat)
-   apply (simp_all add: power_add[symmetric])
-  apply (rule ccontr)
-  apply (simp add: not_less)
-  apply (simp add: le_less[of "2 ^ (64 - obj_bits ko)"])
-  apply (erule disjE)
-   prefer 2
-   apply (clarsimp simp add: power_add[symmetric])
-  apply clarsimp
-  apply (drule mult_less_mono1[of "2 ^ (64 - obj_bits ko)" _ "2 ^ obj_bits ko"])
-   apply (simp add: power_add[symmetric])+
+  apply (metis add.commute is_aligned_mask is_aligned_no_overflow_mask unat_less_2p_word_bits
+               unat_plus_simple)
   done
 
 lemma pspace_aligned_distinct_None':
@@ -415,440 +258,13 @@ lemma n_less_2p_pageBitsForSize:
   for n::machine_word
   apply (subst mult_ac)
   apply (subst shiftl_t2n[symmetric])
-  apply (erule shiftl_less_t2n)
-  using pbfs_less_wb' by (simp add: word_bits_def)
-
-lemma pte_offset_in_datapage:
-  "\<lbrakk> n < 2 ^ (pageBitsForSize sz - pageBits); n \<noteq> 0 \<rbrakk> \<Longrightarrow>
-   (n << pageBits) - (ucast off << pte_bits) < 2 ^ pageBitsForSize sz"
-  for n::machine_word and off::pt_index
-  apply (frule n_less_2p_pageBitsForSize)
-  apply (simp only: bit_simps)
-  apply (subst shiftl_t2n)
-  apply (rule order_le_less_trans[rotated], assumption)
-  apply (rule word_le_imp_diff_le)
-   prefer 2
-   apply (simp add: mult_ac)
-  apply (subst shiftl_t2n[symmetric])
-  apply (subst (asm) mult_ac)
-  apply (subst (asm) shiftl_t2n[symmetric])+
-  apply (rule order_trans[where y="mask pageBits"])
-   apply (simp add: le_mask_shiftl_le_mask[where n=9] ucast_leq_mask pageBits_def)
-  apply word_bitwise
-  apply (clarsimp simp: nth_w2p pageBits_def rev_bl_order_simps)
-  apply (cases sz; simp add: pageBits_def ptTranslationBits_def)
+  apply (erule shiftl_less_t2n[where 'a=machine_word_len, folded word_bits_def])
+  apply (rule pageBitsForSize_bounded)
   done
 
-lemma absHeap_correct:
-  fixes s' :: kernel_state
-  assumes pspace_aligned:  "pspace_aligned s"
-  assumes pspace_distinct: "pspace_distinct s"
-  assumes valid_objs:      "valid_objs s"
-  assumes valid_cur_fpu:   "valid_cur_fpu s"
-  assumes pspace_relation: "pspace_relation (kheap s) (ksPSpace s')"
-  assumes ghost_relation:  "ghost_relation (kheap s) (gsUserPages s') (gsCNodes s')
-                                           (gsPTTypes (ksArchState s'))"
-  assumes arch_state_relation: "(arch_state s, ksArchState s') \<in> arch_state_relation (aobjs_of' s')"
-  shows
-    "absHeap (gsUserPages s') (gsCNodes s') (gsPTTypes (ksArchState s')) (ksPSpace s') (armKSCurFPUOwner (ksArchState s'))
-     = kheap s"
-proof -
-  from ghost_relation
-  have gsUserPages:
-    "\<And>a sz. (\<exists>dev. kheap s a = Some (ArchObj (DataPage dev sz))) \<longleftrightarrow>
-             gsUserPages s' a = Some sz"
-   and gsCNodes:
-    "\<And>a n. (\<exists>cs. kheap s a = Some (CNode n cs) \<and> well_formed_cnode_n n cs) \<longleftrightarrow>
-            gsCNodes s' a = Some n"
-   and gsPTs:
-    "\<And>a pt_t. (\<exists>pt. kheap s a = Some (ArchObj (PageTable pt)) \<and> pt_t = pt_type pt) \<longleftrightarrow>
-               gsPTTypes (ksArchState s') a = Some pt_t"
-    by (fastforce simp add: ghost_relation_def)+
-
-  show "?thesis"
-    supply image_cong_simp [cong del]
-    apply (rule ext)
-    apply (simp add: absHeap_def split: option.splits)
-    apply (rule conjI)
-    using pspace_relation
-     apply (clarsimp simp: pspace_relation_def pspace_dom_def UNION_eq dom_def Collect_eq)
-     apply (erule_tac x=x in allE)
-     apply clarsimp
-     apply (case_tac "kheap s x", simp)
-     apply (erule_tac x=x in allE, clarsimp)
-     apply (erule_tac x=x in allE, simp add: Ball_def)
-     apply (erule_tac x=x in allE, clarsimp)
-     apply (rename_tac a)
-     apply (case_tac a; simp add: other_obj_relation_def
-                             split: if_split_asm Structures_H.kernel_object.splits)
-      apply (rename_tac sz cs)
-      apply (clarsimp simp: image_def cte_map_def well_formed_cnode_n_def Collect_eq dom_def)
-      apply (erule_tac x="replicate sz False" in allE)+
-      apply simp
-     apply (rename_tac arch_kernel_obj)
-     apply (case_tac arch_kernel_obj; simp add: image_def)
-      apply (erule allE, drule_tac x=0 in bspec, simp, fastforce)
-     apply (erule_tac x=0 in allE, simp add: not_less)
-     apply (rename_tac vmpage_size)
-     apply (case_tac vmpage_size; simp add: bit_simps)
-
-    apply (clarsimp split: kernel_object.splits)
-    apply (intro conjI impI allI)
-           apply (erule pspace_dom_relatedE[OF _ pspace_relation])
-           apply clarsimp
-           apply (case_tac ko; simp add: tcb_relation_cut_def other_obj_relation_def)
-             apply (clarsimp simp: cte_relation_def split: if_split_asm)
-            apply (clarsimp simp: ep_relation_def EndpointMap_def
-                            split: Structures_A.endpoint.splits)
-           apply (clarsimp simp: EndpointMap_def split: Structures_A.endpoint.splits)
-           apply (rename_tac arch_kernel_obj)
-           apply (case_tac arch_kernel_obj; simp add: other_obj_relation_def)
-            apply (clarsimp simp add: pte_relation_def)
-           apply (clarsimp split: if_split_asm)+
-
-          apply (erule pspace_dom_relatedE[OF _ pspace_relation])
-          apply (case_tac ko; simp add: tcb_relation_cut_def other_obj_relation_def)
-            apply (clarsimp simp: cte_relation_def split: if_split_asm)
-           apply (clarsimp simp: ntfn_relation_def AEndpointMap_def
-                           split: Structures_A.ntfn.splits)
-          apply (clarsimp simp: AEndpointMap_def split: Structures_A.ntfn.splits)
-          apply (rename_tac arch_kernel_obj)
-          apply (case_tac arch_kernel_obj; simp add: other_obj_relation_def)
-           apply (clarsimp simp add: pte_relation_def)
-          apply (clarsimp split: if_split_asm)+
-
-         apply (erule pspace_dom_relatedE[OF _ pspace_relation])
-         apply (case_tac ko; simp add: tcb_relation_cut_def other_obj_relation_def)
-          apply (clarsimp simp: cte_relation_def split: if_split_asm)
-         apply (rename_tac arch_kernel_obj)
-         apply (case_tac arch_kernel_obj; simp add: other_obj_relation_def)
-          apply (clarsimp simp add: pte_relation_def)
-         apply (clarsimp split: if_split_asm)+
-
-        apply (erule pspace_dom_relatedE[OF _ pspace_relation])
-        apply (case_tac ko, simp_all add: tcb_relation_cut_def other_obj_relation_def)
-         apply (clarsimp simp add: cte_relation_def split: if_split_asm)
-        apply (rename_tac arch_kernel_obj)
-        apply (case_tac arch_kernel_obj, simp_all add: other_obj_relation_def)
-         apply (clarsimp simp add: pte_relation_def)
-        apply (rename_tac vmpage_size)
-        apply (cut_tac a=y and sz=vmpage_size in gsUserPages, clarsimp split: if_split_asm)
-        apply (case_tac "n=0", simp)
-        apply (case_tac "kheap s (y + n * 2 ^ pageBits)")
-         apply (rule ccontr)
-         apply (clarsimp simp: shiftl_t2n mult_ac dest!: gsUserPages[symmetric, THEN iffD1] )
-    using pspace_aligned
-        apply (simp add: pspace_aligned_def dom_def)
-        apply (erule_tac x=y in allE)
-        apply (case_tac "n=0",(simp split: if_split_asm)+)
-        apply (frule (2) unaligned_page_offsets_helper)
-        apply (frule_tac y="n*2^pageBits" in pspace_aligned_distinct_None'
-                                             [OF pspace_aligned pspace_distinct])
-         apply simp
-         apply (rule conjI, clarsimp simp add: word_gt_0)
-         apply (erule n_less_2p_pageBitsForSize)
-        apply (clarsimp simp: shiftl_t2n mult_ac)
-       apply (erule pspace_dom_relatedE[OF _ pspace_relation])
-       apply (case_tac ko, simp_all add: tcb_relation_cut_def other_obj_relation_def)
-        apply (clarsimp simp add: cte_relation_def split: if_split_asm)
-       apply (rename_tac arch_kernel_obj)
-       apply (case_tac arch_kernel_obj, simp_all add: other_obj_relation_def)
-        apply (clarsimp simp add: pte_relation_def)
-       apply (rename_tac vmpage_size)
-       apply (cut_tac a=y and sz=vmpage_size in gsUserPages, clarsimp split: if_split_asm)
-       apply (case_tac "n=0", simp)
-       apply (case_tac "kheap s (y + n * 2 ^ pageBits)")
-        apply (rule ccontr)
-        apply (clarsimp simp: shiftl_t2n mult_ac dest!: gsUserPages[symmetric, THEN iffD1])
-       using pspace_aligned
-       apply (simp add: pspace_aligned_def dom_def)
-       apply (erule_tac x=y in allE)
-       apply (case_tac "n=0",simp+)
-       apply (frule (2) unaligned_page_offsets_helper)
-       apply (frule_tac y="n*2^pageBits" in pspace_aligned_distinct_None'
-                                         [OF pspace_aligned pspace_distinct])
-        apply simp
-        apply (rule conjI, clarsimp simp add: word_gt_0)
-        apply (erule n_less_2p_pageBitsForSize)
-       apply (clarsimp simp: shiftl_t2n mult_ac)
-      apply (erule pspace_dom_relatedE[OF _ pspace_relation])
-      apply (case_tac ko, simp_all add: tcb_relation_cut_def other_obj_relation_def)
-        apply (clarsimp simp add: cte_relation_def split: if_split_asm)
-       prefer 2
-       apply (rename_tac arch_kernel_obj)
-       apply (case_tac arch_kernel_obj, simp_all add: other_obj_relation_def)
-        apply (clarsimp simp add: pte_relation_def)
-       apply (clarsimp split: if_split_asm)
-      apply (clarsimp simp add: TcbMap_def tcb_relation_def valid_obj_def)
-      apply (rename_tac tcb y tcb')
-      apply (case_tac tcb)
-      apply (case_tac tcb')
-      apply (simp add: thread_state_relation_imp_ThStateMap)
-      apply (subgoal_tac "map_option FaultMap (tcbFault tcb) = tcb_fault")
-       prefer 2
-       apply (simp add: fault_rel_optionation_def)
-       using valid_objs[simplified valid_objs_def dom_def fun_app_def, simplified]
-       apply (erule_tac x=y in allE)
-       apply (clarsimp simp: valid_obj_def valid_tcb_def
-                       split: option.splits)
-      using valid_objs[simplified valid_objs_def Ball_def dom_def fun_app_def]
-      apply (erule_tac x=y in allE)
-      using arch_state_relation valid_cur_fpu[simplified valid_cur_fpu_def]
-      apply (erule_tac x=y in allE)
-      apply (clarsimp simp add: cap_relation_imp_CapabilityMap valid_obj_def
-                                valid_tcb_def ran_tcb_cap_cases valid_cap_def2
-                                arch_tcb_relation_imp_ArchTcnMap arch_state_relation_def
-                                is_tcb_cur_fpu_def obj_at_def)
-     apply (simp add: absCNode_def cte_map_def)
-     apply (erule pspace_dom_relatedE[OF _ pspace_relation])
-     apply (case_tac ko, simp_all add: tcb_relation_cut_def other_obj_relation_def
-                                split: if_split_asm)
-      prefer 2
-      apply (rename_tac arch_kernel_obj)
-      apply (case_tac arch_kernel_obj, simp_all add: other_obj_relation_def)
-       apply (clarsimp simp add: pte_relation_def)
-      apply (clarsimp split: if_split_asm)
-     apply (simp add: cte_map_def)
-     apply (clarsimp simp add: cte_relation_def)
-     apply (cut_tac a=y and n=sz in gsCNodes, clarsimp)
-    using pspace_aligned[simplified pspace_aligned_def]
-     apply (drule_tac x=y in bspec, clarsimp)
-     apply clarsimp
-     apply (case_tac "(of_bl ya::machine_word) << cte_level_bits = 0", simp)
-      apply (rule ext)
-      apply simp
-      apply (rule conjI)
-       prefer 2
-    using valid_objs[simplified valid_objs_def Ball_def dom_def
-        fun_app_def]
-       apply (erule_tac x=y in allE)
-       apply (clarsimp simp add: valid_obj_def valid_cs_def valid_cs_size_def
-                   well_formed_cnode_n_def dom_def Collect_eq)
-       apply (frule_tac x=ya in spec, simp)
-       apply (erule_tac x=bl in allE)
-       apply clarsimp+
-      apply (frule pspace_relation_absD[OF _ pspace_relation])
-      apply (simp add: cte_map_def)
-      apply (drule_tac x="y + of_bl bl * 2^cte_level_bits" in spec)
-      apply (clarsimp simp: shiftl_t2n mult_ac)
-      apply (erule_tac x="cte_relation bl" in allE)
-      apply (erule impE)
-       apply (fastforce simp add: well_formed_cnode_n_def)
-      apply clarsimp
-      apply (clarsimp simp add: cte_relation_def)
-      apply (rule cap_relation_imp_CapabilityMap)
-    using valid_objs[simplified valid_objs_def Ball_def dom_def
-        fun_app_def]
-       apply (erule_tac x=y in allE)
-       apply (clarsimp simp: valid_obj_def valid_cs_def valid_cap_def2 ran_def)
-       apply (fastforce simp: cte_level_bits_def objBits_defs)+
-     apply (subgoal_tac "kheap s (y + of_bl ya * 2^cte_level_bits) = None")
-      prefer 2
-    using valid_objs[simplified valid_objs_def Ball_def dom_def fun_app_def]
-      apply (erule_tac x=y in allE)
-      apply (clarsimp simp add: valid_obj_def valid_cs_def valid_cs_size_def)
-      apply (rule pspace_aligned_distinct_None'[OF
-                  pspace_aligned pspace_distinct], assumption)
-      apply (clarsimp simp: word_neq_0_conv power_add cte_index_repair)
-      apply (simp add: well_formed_cnode_n_def dom_def Collect_eq shiftl_t2n mult_ac)
-      apply (erule_tac x=ya in allE)+
-      apply (rule word_mult_less_mono1)
-        apply (subgoal_tac "sz = length ya")
-         apply simp
-         apply (rule of_bl_length, (simp add: word_bits_def)+)[1]
-        apply fastforce
-       apply (simp add: cte_level_bits_def)
-      apply (simp add: word_bits_conv cte_level_bits_def)
-      apply (drule_tac a="2::nat" in power_strict_increasing, simp+)
-     apply (simp add: shiftl_t2n mult_ac)
-     apply (rule ccontr, clarsimp)
-     apply (cut_tac a="y + of_bl ya * 2^cte_level_bits" and n=yc in gsCNodes)
-     apply clarsimp
-
-    (* mapping architecture-specific objects *)
-    apply clarsimp
-    apply (erule pspace_dom_relatedE[OF _ pspace_relation])
-    apply (case_tac ko, simp_all add: tcb_relation_cut_def other_obj_relation_def)
-     apply (clarsimp simp add: cte_relation_def split: if_split_asm)
-    apply (rename_tac arch_kernel_object y ko P arch_kernel_obj)
-    apply (case_tac arch_kernel_object, simp_all add: absHeapArch_def
-                                            split: asidpool.splits)
-
-      apply (in_case "KOASIDPool ?pool")
-      apply clarsimp
-      apply (case_tac arch_kernel_obj)
-         apply (simp add: other_aobj_relation_def asid_pool_relation_def
-                          inv_def o_def)
-        apply (clarsimp simp add:  pte_relation_def)
-       apply (clarsimp simp: other_aobj_relation_def split: if_split_asm)
-      apply (simp add: other_aobj_relation_def)
-
-     apply (in_case "KOPTE ?pte")
-     apply (case_tac arch_kernel_obj;
-            simp add: other_obj_relation_def other_aobj_relation_def asid_pool_relation_def inv_def o_def)
-      apply clarsimp
-      apply (rename_tac p pte pt idx)
-      apply (frule pspace_alignedD, rule pspace_aligned)
-      apply (clarsimp simp add: pte_relation_def)
-      apply (prop_tac "pt_at (pt_type pt) p s", simp add: obj_at_def)
-      apply (drule page_table_at_cross[OF _ pspace_aligned pspace_distinct pspace_relation])
-      apply (clarsimp simp: page_table_at'_def typ_at'_def ko_wp_at'_def)
-      apply (cut_tac a=p and pt_t="pt_type pt" in gsPTs, clarsimp)
-      apply (case_tac "pt_type pt"; clarsimp)
-       apply (in_case "VSRootPT_T")
-       apply (clarsimp simp: absPageTable_def split del: if_split split: option.splits)
-       apply (rule conjI, clarsimp)
-        apply (rule sym)
-        apply (rule pspace_aligned_distinct_None'[OF pspace_aligned pspace_distinct], assumption)
-        apply simp
-        apply (case_tac "idx << pte_bits = 0", simp)
-        apply (clarsimp simp: word_neq_0_conv)
-        apply (rule shiftl_less_t2n)
-         apply (simp add: table_size_def le_mask_iff_lt_2n[THEN iffD1])
-        apply (simp add: table_size_bounded[unfolded word_bits_def, simplified])
-       apply (clarsimp split del: if_split)
-       apply (prop_tac "idx << pte_bits = 0")
-        apply (rename_tac pt_t')
-        apply (cut_tac a="p + (idx << pte_bits)" and pt_t=pt_t' in gsPTs)
-        apply clarsimp
-        apply (rule ccontr)
-        apply (drule_tac y="idx << pte_bits" in pspace_aligned_distinct_None'
-                                                [OF pspace_aligned pspace_distinct])
-         apply (clarsimp simp: word_neq_0_conv table_size_def)
-         apply (rule shiftl_less_t2n, simp)
-          apply (erule order_le_less_trans)
-          apply (simp add: mask_def bit_simps)
-         apply (simp add: bit_simps)
-        apply simp
-       apply (thin_tac "pte_relation' pte pte'" for pte pte')
-       apply (clarsimp simp: pt_bits_def)
-       apply (case_tac pt; clarsimp)
-       apply (rename_tac vs)
-       apply (clarsimp simp: absPageTable0_def)
-       apply (rule conjI, clarsimp)
-        apply (rule ext, rename_tac offs)
-        apply (erule_tac x="ucast offs" in allE, erule impE, rule ucast_leq_mask)
-         apply (simp add: bit_simps)
-        apply (clarsimp dest!: koTypeOf_pte simp: objBits_simps)
-        apply (erule_tac x="ucast offs" in allE)
-        apply clarsimp
-        apply (rename_tac pte y)
-        apply (frule pspace_relation_absD, rule pspace_relation)
-        apply clarsimp
-        apply (drule_tac x="ucast offs" in bspec)
-         apply clarsimp
-         apply (rule ucast_leq_mask)
-         apply (clarsimp simp: bit_simps)
-        apply (clarsimp simp: pte_relation_def ucast_ucast_mask ge_mask_eq vs_index_bits_def)
-        apply (erule pspace_valid_objsE, rule valid_objs)
-        apply (clarsimp simp: valid_obj_def)
-        apply (erule_tac x=offs in allE)
-        apply (clarsimp simp: wellformed_pte_def)
-        apply (case_tac "vs offs"; clarsimp split: if_split_asm)
-         apply (rule set_eqI, simp)
-         apply (rename_tac x, case_tac x; simp)
-        apply (simp add: ucast_ucast_mask ge_mask_eq)
-        apply clarsimp
-        apply (erule_tac x="ucast off" in allE)
-        apply (erule impE)
-         apply (rule ucast_leq_mask)
-         apply (clarsimp simp: bit_simps)
-        apply (clarsimp dest!: koTypeOf_pte simp: objBits_simps)
-        apply (frule pspace_relation_absD, rule pspace_relation)
-        apply clarsimp
-        apply (drule_tac x="ucast off" in bspec)
-         apply clarsimp
-         apply (rule ucast_leq_mask)
-         apply (clarsimp simp: bit_simps)
-        apply (clarsimp simp: pte_relation_def ucast_ucast_mask ge_mask_eq vs_index_bits_def)
-        apply (case_tac "vs off"; simp add: ucast_leq_mask ppn_len_val)
-
-      (* NormalPT_T is an exact duplicate of the VSRootPT_T case, but I don't see any good way
-         to factor out the commonality *)
-      apply (in_case "NormalPT_T")
-      apply (clarsimp simp: absPageTable_def split del: if_split split: option.splits)
-      apply (rule conjI, clarsimp)
-       apply (rule sym)
-       apply (rule pspace_aligned_distinct_None'[OF pspace_aligned pspace_distinct], assumption)
-       apply simp
-       apply (case_tac "idx << pte_bits = 0", simp)
-       apply (clarsimp simp: word_neq_0_conv)
-       apply (rule shiftl_less_t2n)
-        apply (simp add: table_size_def le_mask_iff_lt_2n[THEN iffD1])
-       apply (simp add: table_size_bounded[unfolded word_bits_def, simplified])
-      apply (clarsimp split del: if_split)
-      apply (prop_tac "idx << pte_bits = 0")
-       apply (rename_tac pt_t')
-       apply (cut_tac a="p + (idx << pte_bits)" and pt_t=pt_t' in gsPTs)
-       apply clarsimp
-       apply (rule ccontr)
-       apply (drule_tac y="idx << pte_bits" in pspace_aligned_distinct_None'
-                                               [OF pspace_aligned pspace_distinct])
-        apply (clarsimp simp: word_neq_0_conv table_size_def)
-        apply (rule shiftl_less_t2n, simp)
-         apply (erule order_le_less_trans)
-         apply (simp add: mask_def bit_simps)
-        apply (simp add: bit_simps)
-       apply simp
-      apply (thin_tac "pte_relation' pte pte'" for pte pte')
-      apply (clarsimp simp: pt_bits_def)
-      apply (case_tac pt; clarsimp)
-      apply (rename_tac vs)
-      apply (clarsimp simp: absPageTable0_def)
-      apply (rule conjI, clarsimp)
-       apply (rule ext, rename_tac offs)
-       apply (erule_tac x="ucast offs" in allE, erule impE, rule ucast_leq_mask)
-        apply (simp add: bit_simps)
-       apply (clarsimp dest!: koTypeOf_pte simp: objBits_simps)
-       apply (erule_tac x="ucast offs" in allE)
-       apply clarsimp
-       apply (rename_tac pte y)
-       apply (frule pspace_relation_absD, rule pspace_relation)
-       apply clarsimp
-       apply (drule_tac x="ucast offs" in bspec)
-        apply clarsimp
-        apply (rule ucast_leq_mask)
-        apply (clarsimp simp: bit_simps)
-       apply (clarsimp simp: pte_relation_def ucast_ucast_mask ge_mask_eq vs_index_bits_def)
-       apply (erule pspace_valid_objsE, rule valid_objs)
-       apply (clarsimp simp: valid_obj_def)
-       apply (erule_tac x=offs in allE)
-       apply (clarsimp simp: wellformed_pte_def)
-       apply (case_tac "vs offs"; clarsimp split: if_split_asm)
-        apply (rule set_eqI, simp)
-        apply (rename_tac x, case_tac x; simp)
-       apply (simp add: ucast_ucast_mask ge_mask_eq)
-      apply clarsimp
-      apply (erule_tac x="ucast off" in allE)
-      apply (erule impE)
-       apply (rule ucast_leq_mask)
-       apply (clarsimp simp: bit_simps)
-      apply (clarsimp dest!: koTypeOf_pte simp: objBits_simps)
-      apply (frule pspace_relation_absD, rule pspace_relation)
-      apply clarsimp
-      apply (drule_tac x="ucast off" in bspec)
-       apply clarsimp
-       apply (rule ucast_leq_mask)
-       apply (clarsimp simp: bit_simps)
-      apply (clarsimp simp: pte_relation_def ucast_ucast_mask ge_mask_eq vs_index_bits_def)
-      apply (case_tac "vs off"; simp add: ucast_leq_mask ppn_len_val)
-
-     apply (in_case "DataPage ?p ?sz")
-     apply (clarsimp split: if_splits)
-
-    apply (in_case "KOVCPU ?vcpu")
-    apply clarsimp
-    apply (rename_tac arch_kernel_obj vcpu)
-    apply (case_tac arch_kernel_obj;
-           clarsimp simp: other_obj_relation_def other_aobj_relation_def pte_relation_def split: if_splits)
-    apply (rename_tac vcpu')
-    apply (case_tac vcpu')
-    apply (clarsimp simp: vcpu_relation_def split: vcpu.splits)
-    done
-qed
-
-text \<open>The following function can be used to reverse cte_map.\<close>
-definition
+text \<open>The following function can be used to reverse cte_map. The 3 originates from tcb_cnode_index,
+  which is the smallest size word which can contain all the cap indices in a TCB's CNode.\<close>
+definition cteMap :: "(obj_ref \<rightharpoonup> nat) \<Rightarrow> obj_ref \<Rightarrow> cslot_ptr" where
   "cteMap cns \<equiv> \<lambda>p.
      let P = (\<lambda>(a,bl). cte_map (a,bl) = p \<and> cns a = Some (length bl))
      in if \<exists>x. P x
@@ -893,12 +309,35 @@ proof -
   from rel have gsCNodes:
     "\<forall>a n. (\<exists>cs. kheap s a = Some (CNode n cs) \<and> well_formed_cnode_n n cs) \<longleftrightarrow>
            gsCNodes s' a = Some n"
-    by (simp add: state_relation_def ghost_relation_def)
+    by (clarsimp simp: state_relation_def simp flip: cns_of_heap_Some
+                 dest!: ghost_relation_wrapper_genD)
+
+  (* arch-split: selection of helpers with same proof on all architectures due to the definitions
+     of these constants being available even in generic theories; 3 is size of cte_ref inside a TCB
+     CNode, and 8 = 2^3. *)
+
+  have cte_level_bits3_helper:
+    "3 + cte_level_bits \<le> tcbBlockSizeBits"
+    by (simp add: tcbBlockSizeBits_def cte_level_bits_def)
+
+  have cte_level_bits8_2p_helper:
+    "8 * 2 ^ cte_level_bits < (2::machine_word) ^ tcbBlockSizeBits - 1"
+    by (simp add: tcbBlockSizeBits_def cte_level_bits_def)
+
+  have cte_level_bits8_nat_helper:
+    "8 * (2::nat) ^ cte_level_bits < 2 ^ word_bits"
+    by (simp add: word_bits_conv cte_level_bits_def)
+
+  have cte_level_bits8_unat_nat_helper:
+    "8 * unat ((2::machine_word) ^ cte_level_bits) < 2 ^ word_bits"
+    by (simp add: word_bits_conv cte_level_bits_def)
+
   show ?thesis
-  apply (simp add: dom_def cteMap_def  split: if_split_asm)
+  apply (simp add: dom_def cteMap_def split: if_split_asm)
   apply (clarsimp simp: caps_of_state_cte_wp_at split: if_split_asm)
   apply (drule cte_wp_cte_at)
   apply (intro conjI impI)
+   (* address is a CNode *)
    apply (rule some_equality)
     apply (clarsimp simp add: split_def)
     apply (frule gsCNodes[rule_format,THEN iffD2])
@@ -912,9 +351,11 @@ proof -
    apply (frule (1) cte_at_CNodeI)
    apply (frule (2) cte_map_inj_eq[OF _ _ _ valid_objs pspace_aligned pspace_distinct])
    apply clarsimp
+  (* address is in a TCB's cnode *)
   apply (case_tac p)
-  apply (clarsimp simp add: cte_wp_at_cases)
+  apply (clarsimp simp: cte_wp_at_cases)
   apply (erule disjE)
+   apply (subgoal_tac "False", simp)
    apply clarsimp
    apply (drule_tac x=a in spec, drule_tac x=b in spec, simp)
    apply (cut_tac a=a and n=sz in gsCNodes[rule_format])
@@ -929,59 +370,79 @@ proof -
   using pspace_aligned'[simplified pspace_aligned'_def]
   apply (drule_tac x=a in bspec, simp add: dom_def)
   apply (simp add: objBitsKO_def cte_map_def)
+  apply (drule tcb_cap_cases_length)
+  (* avoid leaking LENGTH *)
+  apply (frule_tac b=b and c=cte_level_bits in bin_to_bl_of_bl_eq[where 'a=machine_word_len, folded word_bits_def])
+    apply (simp add: cte_level_bits3_helper)
+   using obj_sizeBits_less_word_bits cte_level_bits3_helper
+   apply simp
   apply (rule conjI[rotated])
-   apply (drule tcb_cap_cases_length)
-   apply (frule_tac b=b and c=cte_level_bits in bin_to_bl_of_bl_eq)
-     apply (fastforce simp: cte_level_bits_def objBits_defs shiftl_t2n mult_ac)+
+   apply (fastforce simp: shiftl_t2n mult_ac) (* obj_ref part *)
+  (* cap_ref part *)
   apply (case_tac "b = [False, False, False]")
    apply simp
-  apply (frule_tac b=b and c=cte_level_bits in bin_to_bl_of_bl_eq)
-    apply (fastforce simp: tcb_cap_cases_length cte_level_bits_def objBits_defs)+
-  apply (subgoal_tac "ksPSpace s' (cte_map (a, b)) = None")
-   prefer 2
+  apply (prop_tac "ksPSpace s' (cte_map (a, b)) = None")
    apply (rule ccontr)
    apply clarsimp
-  using pspace_distinct'[simplified pspace_distinct'_def]
+   using pspace_distinct'[simplified pspace_distinct'_def]
    apply (drule_tac x=a in bspec, simp add: dom_def)
    apply (simp add: ps_clear_def dom_def mask_2pm1[symmetric] x_power_minus_1)
    apply (simp add: objBitsKO_def)
    apply (drule_tac a="cte_map (a, b)" in equals0D)
    apply (clarsimp simp add: cte_map_def)
-   apply (drule tcb_cap_cases_length)
    apply (erule impE)
     apply (rule word_plus_mono_right)
-     apply (cut_tac 'a=machine_word_len and xs=b in of_bl_length, fastforce simp: word_bits_conv)
-     apply (drule_tac k="2^cte_level_bits" in word_mult_less_mono1)
-       apply (fastforce simp: cte_level_bits_def objBits_defs)+
+     apply (cut_tac 'a=machine_word_len and xs=b in of_bl_length, fastforce)
+     (* avoid leaking LENGTH *)
+     apply (drule_tac k="2^cte_level_bits" in word_mult_less_mono1[where 'a=machine_word_len, folded word_bits_def])
+       apply (simp only: zero_one_less_2p_SizeBits[simplified cteSizeBits_cte_level_bits])
+      using obj_sizeBits_less_word_bits cte_level_bits3_helper
+      apply simp
+      apply (simp add: cte_level_bits8_nat_helper)
      apply (simp add: mask_def)
      apply (rule ccontr)
      apply (simp add: not_le shiftl_t2n mult_ac)
-     apply (drule (1) less_trans, fastforce simp: cte_level_bits_def objBits_defs)
+     apply (drule (1) less_trans)
+     using cte_level_bits8_2p_helper
+     apply simp
     apply (drule is_aligned_no_overflow'[simplified mask_2pm1[symmetric]])
-    apply (simp add: word_bits_conv)
-   apply simp
+    apply simp
    apply (erule impE)
     apply (drule is_aligned_no_overflow'[simplified mask_2pm1[symmetric]])
-    apply (cut_tac 'a=machine_word_len and xs=b in of_bl_length, simp add: word_bits_conv)
-    apply (drule_tac k="2^cte_level_bits" in word_mult_less_mono1)
-      apply (fastforce simp: cte_level_bits_def objBits_defs)+
+    apply (cut_tac 'a=machine_word_len and xs=b in of_bl_length, simp)
+    (* avoid leaking LENGTH *)
+    apply (drule_tac k="2^cte_level_bits" in word_mult_less_mono1[where 'a=machine_word_len, folded word_bits_def])
+      apply (simp only: zero_one_less_2p_SizeBits[simplified cteSizeBits_cte_level_bits])
+     apply simp
+     using cte_level_bits8_unat_nat_helper
+     apply simp
     apply (erule word_random)
     apply (rule order.strict_implies_order)
     apply (simp add: shiftl_t2n mult_ac)
     apply (erule less_trans)
-    apply (fastforce simp: cte_level_bits_def objBits_defs mask_def)
+    apply (simp add: mask_def cte_level_bits8_2p_helper)
    apply (simp add: mult.commute[of _ "2^cte_level_bits"]
                     shiftl_t2n[of _ cte_level_bits, simplified, symmetric])
-   apply word_bitwise
-   apply simp
    apply (case_tac b, simp)
    apply (rename_tac b, case_tac b, simp)
    apply (rename_tac b, case_tac b, simp)
-   apply (clarsimp simp add: test_bit_of_bl eval_nat_numeral cte_level_bits_def)
+   using obj_sizeBits_less_word_bits cte_level_bits3_helper
+   apply clarsimp
+   (* since one of the bits of the cap ref is set, of_bl can't be 0, so shifting it left can't be 0 *)
+   (* avoid leaking LENGTH *)
+   apply (subst (asm) word_shift_nonzero[where 'a=machine_word_len and m=3 and n=cte_level_bits,
+                                         folded word_bits_def])
+      apply (rule order.strict_implies_order)
+      apply (rule of_bl_length_less[where 'a=machine_word_len, folded word_bits_def]; simp)
+     apply simp
+    apply (subst of_bl_0[where n=3, symmetric])
+    (* we have only 3 bits, explore all cases *)
+    apply (case_tac aa; case_tac ab; case_tac ac; simp)
+   apply simp
   apply (simp add: cte_map_def shiftl_t2n mult_ac split: option.splits)
-  apply (drule tcb_cap_cases_length)
-  apply (rule of_bl_mult_and_not_mask_eq[where m=cte_level_bits, simplified])
-   apply (fastforce simp: cte_level_bits_def objBits_defs)+
+  apply (erule of_bl_mult_and_not_mask_eq[where m=cte_level_bits, simplified])
+  apply simp
+  apply (simp add: cte_level_bits3_helper)
   done
 qed
 
@@ -1049,7 +510,7 @@ proof -
     apply (case_tac cte, clarsimp)
     apply (case_tac aa, simp_all)
     apply (rename_tac arch_cap)
-    apply (case_tac arch_cap, simp_all)
+    apply clarsimp
     done
 qed
 
@@ -1265,7 +726,6 @@ qed
 lemmas absCDT_correct = absCDT_correct'(1)
 lemmas cdt_simple_rel =  absCDT_correct'(2)
 
-
 (* Produce a cdt_list from a cdt by sorting the children
    sets by reachability via mdbNext. We then demonstrate
    that a list satisfying the state relation must
@@ -1276,8 +736,6 @@ definition sort_cdt_list where
   "sort_cdt_list cd m =
      (\<lambda>p. THE xs. set xs = {c. cd c = Some p} \<and>
                   partial_sort.psorted (\<lambda>x y. m \<turnstile> cte_map x \<leadsto>\<^sup>* cte_map y) xs \<and> distinct xs)"
-
-end
 
 locale partial_sort_cdt =
   partial_sort "\<lambda> x y.  m' \<turnstile> cte_map x \<leadsto>\<^sup>* cte_map y"
@@ -1293,8 +751,6 @@ locale partial_sort_cdt =
   assumes assms' : "pspace_aligned s" "pspace_distinct s" "pspace_aligned' s'"
                    "pspace_distinct' s'" "valid_objs s" "valid_mdb s" "valid_list s"
 begin
-
-interpretation Arch . (*FIXME: arch-split*)
 
 lemma valid_list_2 : "valid_list_2 t m"
   apply (insert assms')
@@ -1477,9 +933,7 @@ lemma sort_cdt_list_correct:
   apply (simp add: valid_list_def t_def m_def del: split_paired_All)
   done
 
-end
-
-context begin interpretation Arch . (*FIXME: arch-split*)
+end (* partial_sort_cdt *)
 
 definition absCDTList where
   "absCDTList cnp h \<equiv> sort_cdt_list (absCDT cnp h) h"
@@ -1578,31 +1032,6 @@ lemma absInterruptStates_correct:
   apply (clarsimp split: irq_state.splits irqstate.splits)
   done
 
-definition
-  "absArchState s' aobjs' \<equiv>
-   case s' of
-     ARMKernelState asid_tbl kvspace vmid_tab next_vmid global_us_vspace current_vcpu
-                    num_list_regs gs_pt_types current_fpu_owner \<Rightarrow>
-     \<lparr> arm_asid_table = asid_tbl \<circ> ucast,
-       arm_kernel_vspace = kvspace,
-       arm_asid_map = armKSASIDMap' s' aobjs',
-       arm_vmid_table = map_option ucast \<circ> vmid_tab,
-       arm_next_vmid = next_vmid,
-       arm_us_global_vspace = global_us_vspace,
-       arm_current_vcpu = current_vcpu,
-       arm_gicvcpu_numlistregs = num_list_regs,
-       arm_current_fpu_owner = current_fpu_owner \<rparr>"
-
-lemma absArchState_correct:
-  "(s,s') \<in> state_relation \<Longrightarrow> absArchState (ksArchState s') (aobjs_of' s') = arch_state s"
-  apply (prop_tac "(arch_state s, ksArchState s') \<in> arch_state_relation (aobjs_of' s')")
-   apply (simp add: state_relation_def)
-  apply (clarsimp simp: arch_state_relation_def absArchState_def
-                  split: AARCH64_H.kernel_state.splits)
-  apply (simp add: o_assoc flip: map_option_comp2)
-  apply (simp add: o_def ucast_up_ucast_id is_up map_option.identity)
-  done
-
 definition absSchedulerAction where
   "absSchedulerAction action \<equiv>
     case action of ResumeCurrentThread \<Rightarrow> resume_cur_thread
@@ -1623,12 +1052,12 @@ lemma absExst_correct:
   assumes rel: "(s, s') \<in> state_relation"
   shows "absExst s' = exst s"
   apply (rule det_ext.equality)
-      using rel invs invs'
-      apply (simp_all add: absExst_def absSchedulerAction_correct
-                           absCDTList_correct[THEN fun_cong] state_relation_def invs_def valid_state_def
-                           ready_queues_relation_def invs'_def valid_state'_def
-                           valid_pspace_def valid_sched_def valid_pspace'_def curry_def fun_eq_iff)
-      done
+    using rel invs invs'
+    apply (simp_all add: absExst_def absSchedulerAction_correct
+                         absCDTList_correct[THEN fun_cong] state_relation_def invs_def valid_state_def
+                         ready_queues_relation_def invs'_def valid_state'_def
+                         valid_pspace_def valid_sched_def valid_pspace'_def curry_def fun_eq_iff)
+  done
 
 definition domSchedule_map ::
   "domain_schedule_item list \<Rightarrow> (domain \<times> Structures_A.domain_duration) list"
@@ -1644,9 +1073,21 @@ lemma domSchedule_map_relation:
   "(s, s') \<in> state_relation \<Longrightarrow> domSchedule_map (ksDomSchedule s') = domain_list s"
   by (fastforce elim: domSchedule_map_domain_list_map state_relationE)
 
+locale ADT_H_2 = ADT_H +
+  fixes absHeap ::
+    "(machine_word \<rightharpoonup> vmpage_size) \<Rightarrow> (machine_word \<rightharpoonup> nat) \<Rightarrow>
+     Arch.kernel_state \<Rightarrow> (machine_word \<rightharpoonup> Structures_H.kernel_object) \<Rightarrow> Structures_A.kheap"
+  assumes absHeap_correct:
+    "\<And>s s'.
+     \<lbrakk>pspace_aligned s; pspace_distinct s; valid_objs s; valid_cur_fpu s;
+      pspace_relation (kheap s) (ksPSpace s'); ghost_relation_wrapper s s';
+      (arch_state s, ksArchState s') \<in> arch_state_relation (aobjs_of' s')\<rbrakk>
+     \<Longrightarrow> absHeap (gsUserPages s') (gsCNodes s') (ksArchState s') (ksPSpace s') = kheap s"
+begin
+
 definition
   "absKState s \<equiv>
-   \<lparr>kheap = absHeap (gsUserPages s) (gsCNodes s) (gsPTTypes (ksArchState s)) (ksPSpace s) (armKSCurFPUOwner (ksArchState s)),
+   \<lparr>kheap = absHeap (gsUserPages s) (gsCNodes s) (ksArchState s) (ksPSpace s),
     cdt = absCDT (cteMap (gsCNodes s)) (ctes_of s),
     is_original_cap = absIsOriginalCap (cteMap (gsCNodes s)) (ksPSpace s),
     cur_thread = ksCurThread s, idle_thread = ksIdleThread s,
@@ -1662,7 +1103,6 @@ definition
     interrupt_states = absInterruptStates (ksInterruptState s),
     arch_state = absArchState (ksArchState s) (aobjs_of' s),
     exst = absExst s\<rparr>"
-
 
 definition checkActiveIRQ :: "(kernel_state, bool) nondet_monad" where
   "checkActiveIRQ \<equiv>
@@ -1732,6 +1172,6 @@ definition ADT_H ::
       Fin = \<lambda>((tc,s),m,e). ((tc, absKState s),m,e),
       Step = (\<lambda>u. global_automaton check_active_irq_H (do_user_op_H uop) kernel_call_H)\<rparr>"
 
-end
+end (* ADT_H_2 *)
 
 end
